## *Mathematics forumlate by Coq. Coq is a formal system.

```coq
Inductive nat : Type :=
| zero : nat
| succ : nat -> nat.

Fixpoint add (m n : nat) : nat :=
  match m with
  | zero => n
  | succ m' => succ (add m' n)
  end.

Theorem one_plus_one : add (succ zero) (succ zero) = succ (succ zero).
Proof.
  simpl.
  reflexivity.
Qed.

```

## To prove \( 1 + 1 = 2 \) using **Church numerals**, we will use the formalism of numbers in lambda calculus. In this system, natural numbers are represented as higher-order functions, and addition is defined through functional composition.

---

### **Church Numerals**
1. **Definition of Church Numerals**:
   - \( 0 \): \( \lambda f . \lambda x . x \)  
     (Applies \( f \) zero times to \( x \)).
   - \( 1 \): \( \lambda f . \lambda x . f(x) \)  
     (Applies \( f \) once to \( x \)).
   - \( 2 \): \( \lambda f . \lambda x . f(f(x)) \)  
     (Applies \( f \) twice to \( x \)).
   - In general, \( n \): \( \lambda f . \lambda x . f^n(x) \)  
     (Applies \( f \) \( n \)-times to \( x \)).

2. **Addition in Church Numerals**:
   Addition of Church numerals \( m \) and \( n \) is defined as:
   \[
   \text{Add} = \lambda m . \lambda n . \lambda f . \lambda x . m(f)(n(f)(x))
   \]
   This says: "Apply \( m \)-times function \( f \), starting with \( n(f)(x) \)."

---

### **Prove \( 1 + 1 = 2 \)**

#### Step 1: Represent \( 1 \) and \( 2 \)
- \( 1 = \lambda f . \lambda x . f(x) \)
- \( 2 = \lambda f . \lambda x . f(f(x)) \)

#### Step 2: Apply the Addition Function
\[
\text{Add}(1, 1) = (\lambda m . \lambda n . \lambda f . \lambda x . m(f)(n(f)(x)))(1)(1)
\]

#### Step 3: Expand the Definition
Substitute \( 1 \) for \( m \) and \( n \):
\[
\text{Add}(1, 1) = \lambda f . \lambda x . (1(f)((1(f)(x))))
\]

#### Step 4: Substitute \( 1 = \lambda f . \lambda x . f(x) \)
\[
1(f) = \lambda x . f(x)
\]
Substitute into the equation:
\[
\text{Add}(1, 1) = \lambda f . \lambda x . (\lambda x . f(x))(f(x))
\]

#### Step 5: Evaluate the Inner Function
\[
(\lambda x . f(x))(f(x)) = f(f(x))
\]
Thus:
\[
\text{Add}(1, 1) = \lambda f . \lambda x . f(f(x))
\]

#### Step 6: Recognize the Result
The result \( \lambda f . \lambda x . f(f(x)) \) is the definition of \( 2 \) in Church numerals.

---

### **Conclusion**
Using Church numerals and the addition function, we have shown that:
\[
1 + 1 = 2
\]
in the formal system of lambda calculus. ✅

## on Neumann construction of natural numbers

To rigorously prove \( 1 + 1 = 2 \) using only **brackets**, we can use a formalism based on set theory, where numbers are defined as nested sets. This approach is rooted in the **von Neumann construction of natural numbers**, where:

- \( 0 \) is represented as the empty set: \( 0 = \emptyset \)
- \( 1 \) is the set containing \( 0 \): \( 1 = \{ \emptyset \} \)
- \( 2 \) is the set containing \( 0 \) and \( 1 \): \( 2 = \{ \emptyset, \{ \emptyset \} \} \)
- \( n+1 \) is the successor of \( n \), defined as \( S(n) = n \cup \{ n \} \).

Using this formalism, addition can be derived and \( 1 + 1 = 2 \) can be proved step by step.

---

### **Proof Using Brackets**

#### **Step 1: Definitions**
1. \( 0 = \emptyset \)  
2. \( 1 = \{ \emptyset \} \)  
3. \( 2 = \{ \emptyset, \{ \emptyset \} \} \)

#### **Step 2: Define Addition**
Addition \( a + b \) is defined recursively as:
1. \( a + 0 = a \)
2. \( a + S(b) = S(a + b) \), where \( S(x) = x \cup \{ x \} \) is the successor operation.

---

#### **Step 3: Compute \( 1 + 1 \)**
1. \( 1 + 1 = 1 + S(0) \) (since \( 1 = S(0) \))  
2. By the definition of addition: \( 1 + S(0) = S(1 + 0) \)  
3. Using \( a + 0 = a \): \( 1 + 0 = 1 \)  
4. So, \( S(1 + 0) = S(1) \)  
5. By the definition of \( S(x) \): \( S(1) = 1 \cup \{ 1 \} \)

#### **Step 4: Expand \( S(1) \)**
1. \( 1 = \{ \emptyset \} \)  
2. \( S(1) = 1 \cup \{ 1 \} = \{ \emptyset \} \cup \{ \{ \emptyset \} \} \)  
3. Simplify: \( S(1) = \{ \emptyset, \{ \emptyset \} \} \)  
4. By definition, \( \{ \emptyset, \{ \emptyset \} \} = 2 \).

---

### **Conclusion**
Using only brackets and set-theoretic definitions, we have shown that:
\[
1 + 1 = 2
\]
where the numbers \( 1 \) and \( 2 \) are defined in terms of nested sets. ✅

---

## The proof of \( 1 + 1 = 2 \) is not as trivial as it seems when approached from the perspective of rigorous mathematical foundations. In formal mathematics, particularly in **set theory** and **logic**, this statement requires a precise definition of numbers, addition, and equality.

This proof is famously found in **Principia Mathematica** by Alfred North Whitehead and Bertrand Russell, where \( 1 + 1 = 2 \) is derived as a theorem from axioms and definitions in **Peano arithmetic** and **formal logic**.

---

## **Outline of the Proof**

#### **1. Definition of Numbers**
In Peano arithmetic or set theory:
- \( 0 \) is defined as a base element (often as the empty set \( \emptyset \)).
- Successor function \( S(x) \) defines the next natural number: \( S(0) = 1 \), \( S(1) = 2 \), and so on.
- \( 1 \) is defined as \( S(0) \), and \( 2 \) is defined as \( S(1) \).

---

#### **2. Definition of Addition**
Addition is defined recursively:
1. \( x + 0 = x \) (Base case).
2. \( x + S(y) = S(x + y) \) (Recursive step).

This means that to compute \( 1 + 1 \):
- \( 1 + 1 = 1 + S(0) \)  
- Using the recursive definition: \( 1 + S(0) = S(1 + 0) \)  
- From the base case: \( 1 + 0 = 1 \), so \( S(1 + 0) = S(1) \)  
- By definition of \( S(1) \), \( S(1) = 2 \).

Thus, \( 1 + 1 = 2 \).

---

### **Proof in Principia Mathematica**
In **Principia Mathematica**, the proof appears as *Theorem 54* (written symbolically as \( *54 \)) and follows these steps:

1. Numbers are constructed from formal axioms of logic (specifically, from sets).
2. \( 1 \) and \( 2 \) are rigorously defined using the successor function.
3. Addition is defined recursively.
4. \( 1 + 1 = 2 \) is derived by applying these definitions step by step.

While the process is formally rigorous, the full proof in **Principia Mathematica** spans several pages and is built on a series of earlier theorems and definitions.

---

### **Key Insight**
The statement \( 1 + 1 = 2 \) is intuitively obvious in everyday arithmetic. However, proving it rigorously requires:
1. A formal system (like Peano arithmetic or set theory).
2. Precise definitions of numbers and operations.
3. Logical derivations based on axioms.

This careful foundation ensures that even "simple" arithmetic statements are consistent with the broader structure of mathematics.
